binary-heap: prototype

binary-heap/Heap.v
@@ -1,6 +1,164 @@
-Lemma foo :
-  1 + 1 = 2.
+Require Import Coq.Arith.Arith.
+Require Import Coq.Init.Nat.
+
+Require Import Omega.
+
+(** Simple formalization of an array. *)
+
+Definition array : Set := nat -> nat.
+
+Definition aempty : array := fun _ => 0.
+
+Definition getv (a : array) (k : nat) := a k.
+
+Definition setv (a : array) (k : nat) (v : nat) : array :=
+  fun k' => if k' =? k then v else a k'.
+
+Definition clearv (a : array) (k : nat) : array :=
+  setv a k 0.
+
+Definition swap (a : array) (i j : nat) : array :=
+  let (x, y) := (getv a i, getv a j)
+  in setv (setv a i y) j x.
+
+Lemma array_get_last :
+  forall k v a, getv (setv a k v) k = v.
 Proof.
-  simpl.
+  intros.
+  unfold setv. unfold getv.
+  rewrite <- beq_nat_refl.
   reflexivity.
+Qed.
+
+Hint Rewrite array_get_last.
+
+(** Heap *)
+
+Definition heap : Set := array * nat.
+
+Definition heap_array (h : heap) : array :=
+  match h with
+  | (a, n) => a
+  end.
+
+Definition heap_n (h : heap) : nat :=
+  match h with
+  | (a, n) => n
+  end.
+
+Definition extend_heap (h : heap) (v : nat) : heap :=
+  (setv (heap_array h) (S (heap_n h)) v, S (heap_n h)).
+
+Definition shrink_heap (h : heap) : heap :=
+  match h with
+  | (a, 0) => (a, 0)
+  | (a, S n) => (setv a (S n) 0, n)
+  end.
+
+Definition Heap (h : heap) : Prop :=
+  forall (i : nat),
+    2 <= i /\ i <= heap_n h ->
+    getv (heap_array h) (i/2) >= getv (heap_array h) i.
+
+Fixpoint heap_upify (h : heap) (k dep : nat) : heap :=
+  match dep with
+  | 0 => h
+  | S dep' =>
+      if getv (heap_array h) (k/2) <? getv (heap_array h) (k)
+        then heap_upify (swap (heap_array h) k (k/2), (heap_n h)) (k/2) dep'
+        else h
+  end.
+
+Definition heap_push (h : heap) (v : nat) : heap :=
+  heap_upify (extend_heap h v) (S (heap_n h)) (log2 (S (heap_n h))).
+
+Lemma extend_heap_n :
+  forall (h : heap) (v : nat),
+    heap_n (extend_heap h v) = S (heap_n h).
+Proof.
+  intros. auto.
+Qed.
+
+Lemma heap_upify_correct :
+  forall (h : heap) (k dep : nat),
+    log2 k = dep ->
+    k > 0 ->
+    (forall (i : nat),
+      2 <= i <= heap_n h /\ ~(k = i) -> getv (heap_array h) (i/2) >= getv (heap_array h) i) ->
+    Heap (heap_upify h k dep).
+Proof.
+  intros h k dep.
+  generalize dependent h.
+  generalize dependent k.
+  induction dep.
+  - intros.
+    rewrite Nat.log2_null in H.
+    assert (k = 1). { omega. }
+    clear H H0.
+    subst. simpl.
+    unfold Heap. intros.
+    assert (1 <> i). { omega. }
+    auto.
+  - intros. unfold heap_upify. fold heap_upify.
+    destruct (getv (heap_array h) (k / 2) <? getv (heap_array h) k) eqn:H2.
+    + rewrite Nat.ltb_lt in H2.
+      apply IHdep.
+      * admit.
+      * admit.
+      * intros. destruct H3.
+        admit.
+    + rewrite Nat.ltb_ge in H2.
+      unfold Heap.
+      intros.
+      destruct (k =? i) eqn:H4.
+      * apply beq_nat_true in H4. subst.
+        apply H2.
+      * apply beq_nat_false in H4.
+        apply H1. auto.
+  Admitted.
+
+Lemma extend_heap_unaffected :
+  forall (i v : nat) (h : heap),
+    1 <= i <= heap_n h ->
+    getv (heap_array (extend_heap h v)) i = getv (heap_array h) i.
+Proof.
+  intros.
+  simpl.
+  unfold setv. unfold getv.
+  destruct (i =? S (heap_n h)) eqn:H1.
+  - apply beq_nat_true in H1. subst. omega.
+  - reflexivity.
+Qed.
+
+Theorem heap_push_correct :
+  forall (h : heap) (v : nat),
+  Heap h -> Heap (heap_push h v).
+Proof.
+  intros.
+  unfold heap_push.
+  apply heap_upify_correct; auto; try omega.
+  intros.
+  rewrite extend_heap_n in H0.
+  destruct H0.
+  unfold Heap in H.
+  assert (2 <= i <= heap_n h).
+  { destruct H0. split. apply H0.
+    rewrite Nat.le_succ_r in H2. destruct H2; auto.
+    subst. exfalso. apply H1. reflexivity. }
+  clear H0 H1.
+  assert (getv (heap_array (extend_heap h v)) (i / 2) = getv (heap_array h) (i / 2)).
+  { apply extend_heap_unaffected.
+    destruct H2. split.
+    - assert (2 / 2 <= i / 2). { apply Nat.div_le_mono. omega. auto. }
+      simpl in H2. simpl. apply H2.
+    - assert (i / 2 <= i / 1). { apply Nat.div_le_compat_l. omega. }
+      eapply Nat.le_trans. apply H2. rewrite Nat.div_1_r. apply H1.
+  }
+  rewrite H0.
+  assert (getv (heap_array (extend_heap h v)) i = getv (heap_array h) i).
+  { apply extend_heap_unaffected.
+    destruct H2. split. omega. apply H2.
+  }
+  rewrite H1.
+  apply H. apply H2.
 Qed.
